@prefix :	<#> .
@prefix rdf:	<http://www.w3.org/1999/02/22-rdf-syntax-ns#> .
@prefix rdfs:	<http://www.w3.org/2000/01/rdf-schema#> .
@prefix xsd:	<http://www.w3.org/2001/XMLSchema#> .
@prefix owl:	<http://www.w3.org/2002/07/owl#> .
@prefix skos:	<http://www.w3.org/2004/02/skos/core#> .
@prefix ldp:	<http://www.w3.org/ns/ldp#> .
@prefix sd:	<http://www.w3.org/ns/sparql-service-description#> .
@prefix dc:	<http://purl.org/dc/elements/1.1/> .
@prefix dct:	<http://purl.org/dc/terms/> .
@prefix lda:	<http://purl.org/linked-data/api/vocab#> .
@prefix sp:	<http://spinrdf.org/sp#> .
@prefix spin:	<http://spinrdf.org/spin#> .
@prefix void:	<http://rdfs.org/ns/void#> .
@prefix sioc:	<http://rdfs.org/sioc/ns#> .
@prefix foaf:	<http://xmlns.com/foaf/0.1/> .
@prefix gc:     <http://client.graphity.org/ontology#> .
@prefix gp:	<http://processor.graphity.org/ontology#> .
@prefix srv:    <http://jena.hpl.hp.com/Service#> .

: a owl:Ontology ;
    owl:imports gp:, lda: , void:, foaf: ;
    dct:title "Sitemap" ;
    rdfs:label "Sitemap" ;
    dct:description "Default sitemap for SPARQL service" ;
    dct:created "2013-03-09T13:53:00+03:00"^^xsd:dateTime ;
    dct:modified "2013-08-06T23:39:00+03:00"^^xsd:dateTime ;
    foaf:isPrimaryTopicOf <ontology> ;
    rdfs:seeAlso <sparql> .

<service#this> a sd:Service ;
    foaf:isPrimaryTopicOf <service> ;
    dct:title "Graphity Client endpoint" ;
    sd:endpoint <sparql> ;
    gp:graphStore <service> ;
    # srv:queryAuthUser "username" ;
    # srv:queryAuthPwd "password" ;
    sd:supportedLanguage sd:SPARQL11Query ;
    sd:defaultDataset [ a sd:Dataset ;
	    sd:defaultGraph <dataset#this>
	] .

<dataset#this> a sd:Graph, void:Dataset ;
    dct:title "Graphity Client dataset" ;
    foaf:isPrimaryTopicOf <dataset> ;
    rdfs:isDefinedBy : ;
    void:triples "494"^^xsd:integer ;
    void:sparqlEndpoint <sparql> .

# EXTERNAL

ldp:pageOf a owl:ObjectProperty ;
    rdfs:domain ldp:Page ;
    rdfs:range ldp:Container ;
    rdfs:isDefinedBy ldp: .

lda:ItemEndpoint a owl:Class .
lda:ListEndpoint a owl:Class.

void:inDataset a owl:ObjectProperty ;
    rdfs:domain foaf:Document ;
    rdfs:range void:Dataset ;
    rdfs:isDefinedBy void: .

# RESOURCES

<.> a sioc:Site, ldp:Container, foaf:Document ;
    dct:title "Graphity Client" ;
    dct:description "Generic Linked Data browser and end-user-oriented platform" ;
    foaf:logo <static/img/graphity-logo.svg> ;
    foaf:maker <http://graphityhq.com/#company> ;
    gc:stylesheet <static/org/graphity/client/xsl/global-xhtml.xsl> ;
    gp:service <service#this> ;
    rdfs:isDefinedBy : ;
    void:inDataset <dataset#this> ;
    rdfs:seeAlso : , <sparql>, <http://graphityhq.com>, <http://semantic-web.dk> .

<ontology> a foaf:Document, sioc:Item ;
    sioc:has_container <.> ;
    dct:title "Ontology document" ;
    foaf:primaryTopic : ;
    rdfs:isDefinedBy : ;
    void:inDataset <dataset#this> .

<dataset> a foaf:Document, sioc:Item ;
    sioc:has_container <.> ;
    dct:title "Dataset document" ;
    foaf:primaryTopic <dataset#this> ;
    rdfs:isDefinedBy : ;
    void:inDataset <dataset#this> .

<service> a foaf:Document, sioc:Item ;
    sioc:has_container <.> ;
    dct:title "Service document" ;
    foaf:primaryTopic <service#this> ;
    rdfs:isDefinedBy : ;
    void:inDataset <dataset#this> .

<resources> a ldp:Container, sioc:Container, foaf:Document ;
    sioc:has_space <.> ;
    dct:title "Resources" ;
    rdfs:isDefinedBy : ;
    void:inDataset <dataset#this> .

<instances> a ldp:Container, sioc:Container, foaf:Document ;
    sioc:has_space <.> ;
    dct:title "Instances" ;
    rdfs:isDefinedBy : ;
    void:inDataset <dataset#this> .

<ontologies> a ldp:Container, sioc:Container, foaf:Document ;
    sioc:has_space <.> ;
    dct:title "Ontologies" ;
    rdfs:isDefinedBy : ;
    void:inDataset <dataset#this> .

<classes> a ldp:Container, sioc:Container, foaf:Document ;
    sioc:has_space <.> ;
    dct:title "Classes" ;
    rdfs:isDefinedBy : ;
    void:inDataset <dataset#this> .

<datasets> a ldp:Container, sioc:Container, foaf:Document ;
    sioc:has_space <.> ;
    dct:title "Datasets" ;
    rdfs:isDefinedBy : ;
    void:inDataset <dataset#this> .

<services> a ldp:Container, sioc:Container, foaf:Document ;
    sioc:has_space <.> ;
    dct:title "Services" ;
    rdfs:isDefinedBy : ;
    void:inDataset <dataset#this> .

<queries> a ldp:Container, sioc:Container, foaf:Document ;
    sioc:has_space <.> ;
    dct:title "Queries" ;
    rdfs:isDefinedBy : ;
    void:inDataset <dataset#this> .

<resources/labelled> a ldp:Container, foaf:Document ;
    sioc:has_space <resources> ;
    dct:title "Labelled resources" ;
    rdfs:isDefinedBy : ;
    void:inDataset <dataset#this> .

<properties/labelled> a ldp:Container, foaf:Document ;
    sioc:has_space <properties> ;
    dct:title "Labelled properties" ;
    rdfs:isDefinedBy : ;
    void:inDataset <dataset#this> .

<sparql> a foaf:Document ;
    dct:title "SPARQL endpoint" ;
    rdfs:isDefinedBy : ;
    void:inDataset <dataset#this> .

# RESOURCE CLASSES

<classes/resource> a foaf:Document, sioc:Item ;
    sioc:has_container <classes> ;
    foaf:primaryTopic <classes/resource#this> ;
    rdfs:isDefinedBy : ;
    void:inDataset <dataset#this> .

<classes/resource#this> a owl:Class ;
    foaf:isPrimaryTopicOf <classes/resource> ;
    rdfs:subClassOf foaf:Document ,
	[ a owl:Restriction ;
		owl:onProperty lda:uriTemplate ;
		owl:hasValue "/{path: .*}"
	] ;
    spin:query [ a :DescribeTemplate ] ;
    rdfs:label "Resource" ;
    rdfs:comment "Catch-all resource class (template)" ;
    rdfs:isDefinedBy : ;
    void:inDataset <dataset#this> .

# ====

<classes/ontology-doc> a foaf:Document, sioc:Item ;
    sioc:has_container <classes> ;
    foaf:primaryTopic <classes/ontology-doc#this> ;
    rdfs:isDefinedBy : ;
    void:inDataset <dataset#this> .

<classes/ontology-doc#this> a owl:Class ;
    foaf:isPrimaryTopicOf <classes/ontology-doc> ;
    rdfs:subClassOf foaf:Document ,
	[ a owl:Restriction ;
		owl:onProperty lda:uriTemplate ;
		owl:hasValue "/ontology"
	] ;
    spin:query [ a gp:ConstructResourcesTemplate ] ;
    rdfs:label "Ontology document resource" ;
    rdfs:isDefinedBy : ;
    void:inDataset <dataset#this> .

# ====

:LabelledResourceContainer a owl:Class ;
        rdfs:subClassOf foaf:Document, ldp:Container, lda:ListEndpoint ,
	[ a owl:Restriction ;
		owl:onProperty lda:uriTemplate ;
		owl:hasValue "/resources/labelled"
	] ;
    spin:query [ a gp:DescribeLabelResourcesTemplate ] ;
    rdfs:label "Labelled resource container" ;
    rdfs:isDefinedBy : ;
    void:inDataset <dataset#this> .

# ====

:LabelledPropertyContainer a owl:Class, gp:Template ;
    rdfs:subClassOf foaf:Document, ldp:Page, lda:ListEndpoint ,
	[ a owl:Restriction ;
		owl:onProperty void:inDataset ;
		owl:hasValue <dataset#this>
	] ,
	[ a owl:Restriction ;
		owl:onProperty lda:uriTemplate ;
		owl:hasValue "/properties/labelled"
	] ;
    spin:query [ a gp:DescribeLabelPropertiesTemplate ] ;
    rdfs:label "Labelled properties container" ;
    rdfs:isDefinedBy : ;
    void:inDataset <dataset#this> .

# DATASETS & SERVICES

<datasets/DBPedia> a foaf:Document, sioc:Item ;
    sioc:has_container <datasets> ;
    foaf:primaryTopic <datasets/DBPedia#this> ;
    rdfs:isDefinedBy : ;
    void:inDataset <dataset#this> .

<datasets/DBPedia#this> a void:Dataset ;
    foaf:isPrimaryTopicOf <datasets/DBPedia> ;
    dct:title "DBPedia" ;
    dct:description "RDF data extracted from Wikipedia" ;
    foaf:homepage <http://dbpedia.org> ;
    foaf:logo <http://wiki.dbpedia.org/images/dbpedia_logo.png> ;
    void:sparqlEndpoint <http://dbpedia.org/sparql> ;
    void:exampleResource <http://dbpedia.org/resource/Berlin>,
	<http://dbpedia.org/resource/Physics>,
	<http://dbpedia.org/resource/Ludwig_van_Beethoven> ;
    void:uriSpace "http://dbpedia.org/resource/" ;
    void:triples "550000000"^^xsd:integer .
[ a sd:Service ;
    sd:endpoint <http://dbpedia.org/sparql> ;
    sd:supportedLanguage sd:SPARQL11Query ] .

# ====

<datasets/Enipedia> a foaf:Document, sioc:Item ;
    sioc:has_container <datasets> ;
    foaf:primaryTopic <datasets/Enipedia#this> ;
    rdfs:isDefinedBy : ;
    void:inDataset <dataset#this> .

<datasets/Enipedia#this> a void:Dataset ;
    foaf:isPrimaryTopicOf <datasets/Enipedia> ;
    dct:title "Enipedia" ;
    dct:description "Enipedia is an active exploration into the applications of wikis and the semantic web for energy and industry issues" ;
    foaf:homepage <http://enipedia.tudelft.nl/wiki/Enipedia> ;
    foaf:logo <http://enipedia.tudelft.nl/enipedia/images/b/bd/eni.png> ;
    void:sparqlEndpoint <http://enipedia.tudelft.nl/sparql/> ;
    void:triples "4317758"^^xsd:integer .
[ a sd:Service ;
    sd:endpoint <http://enipedia.tudelft.nl/sparql/> ] .

# ====

<datasets/OpenEI> a foaf:Document, sioc:Item ;
    sioc:has_container <datasets> ;
    foaf:primaryTopic <datasets/OpenEI#this> ;
    rdfs:isDefinedBy : ;
    void:inDataset <dataset#this> .

<datasets/OpenEI#this> a void:Dataset ;
    foaf:isPrimaryTopicOf <datasets/OpenEI> ;
    dct:title "OpenEI" ;
    dct:description "Open Energy Information (OpenEI) is a knowledge sharing online community dedicated to connecting people with the latest information and data on energy resources from around the world." ;
    foaf:homepage <http://en.openei.org/lod/> ;
    void:sparqlEndpoint <http://en.openei.org/sparql> ;
    void:exampleResource <http://en.openei.org/lod/resource/wiki/Japan> ;
    void:uriSpace "http://en.openei.org/lod/resource/" ;
    void:triples "17231136"^^xsd:integer .
[ a sd:Service ;
    sd:endpoint <http://en.openei.org/sparql> ] .

# ====

<datasets/LinkedGeoData> a foaf:Document, sioc:Item ;
    sioc:has_container <datasets> ;
    foaf:primaryTopic <datasets/LinkedGeoData#this> ;
    rdfs:isDefinedBy : ;
    void:inDataset <dataset#this> .

<datasets/LinkedGeoData#this> a void:Dataset ;
    foaf:isPrimaryTopicOf <datasets/LinkedGeoData> ;
    dct:title "LinkedGeoData" ;
    dct:description "RDF data extracted from OpenStreetMap.org" ;
    foaf:homepage <http://linkedgeodata.org> ;
    foaf:depiction <http://linkedgeodata.org/files/lgdlogo.png> ;
    void:sparqlEndpoint <http://linkedgeodata.org/sparql> ;
    void:exampleResource <http://linkedgeodata.org/triplify/node264695865> ;
    void:uriSpace "http://linkedgeodata.org/triplify/" .
[ a sd:Service ;
    sd:endpoint <http://linkedgeodata.org/sparql> ] .

# ====

_:OrdnanceSurvey a void:Dataset ;
    dct:title "Ordnance Survey" ;
    dct:description "Ordnance Survey is Great Britain's national mapping agency, providing the most accurate and up-to-date geographic data, relied on by government, business and individuals" ;
    foaf:homepage <http://data.ordnancesurvey.co.uk/datasets/os-linked-data> ;
    foaf:logo <http://data.ordnancesurvey.co.uk/img/os-opendata.jpg> ;
    void:sparqlEndpoint <http://data.ordnancesurvey.co.uk/datasets/os-linked-data/apis/sparql> ;
    void:exampleResource <http://data.ordnancesurvey.co.uk/id/postcodeunit/SO164GU> ,
	<http://data.ordnancesurvey.co.uk/id/7000000000037256> ;
    void:uriSpace "http://data.ordnancesurvey.co.uk/id/", "http://data.ordnancesurvey.co.uk/ontology/" .
[ a sd:Service ;
    sd:endpoint <http://data.ordnancesurvey.co.uk/datasets/os-linked-data/apis/sparql> ] .

_:CodePoint a void:Dataset ;
    dct:title "Code-Point Open" ;
    dct:description "Code-Point® Open contains postcode units for Great Britain, each of which has a precise geographic location." ;
    foaf:homepage <http://data.ordnancesurvey.co.uk/datasets/code-point-open> ;
    foaf:logo <http://data.ordnancesurvey.co.uk/img/os-opendata.jpg> ;
    void:sparqlEndpoint <http://data.ordnancesurvey.co.uk/datasets/code-point-open/apis/sparql> ;
    void:exampleResource <http://data.ordnancesurvey.co.uk/id/postcodeunit/SO164GU> ,
	<http://data.ordnancesurvey.co.uk/id/7000000000037256> .
    # void:uriSpace "http://data.ordnancesurvey.co.uk/id/" .
[ a sd:Service ;
    sd:endpoint <http://data.ordnancesurvey.co.uk/datasets/code-point-open/apis/sparql> ] .

_:Eurostat a void:Dataset ;
    dct:title "Eurostat" ;
    dct:description "Detailed statistics on the EU and candidate countries, and various statistical publications for sale" ;
    foaf:homepage <http://epp.eurostat.ec.europa.eu/portal/page/portal/eurostat/home/> ;
    foaf:logo <http://epp.eurostat.ec.europa.eu/portal/page/portal/PGP_ADM_IMAGES/PGE_IMAGES_TEMPLATES/logo.png> ;
    void:sparqlEndpoint <http://www4.wiwiss.fu-berlin.de/eurostat/sparql> ;
    void:exampleResource <http://www4.wiwiss.fu-berlin.de/eurostat/resource/countries/Danmark> ;
    void:uriSpace "http://www4.wiwiss.fu-berlin.de/eurostat/resource/" ;
    void:triples "8850"^^xsd:integer .
[ a sd:Service ;
    sd:endpoint <http://www4.wiwiss.fu-berlin.de/eurostat/sparql> ] .

_:UKStatistics a void:Dataset ;
    dct:title "UK Statistics" ;
    dct:description "This site contains Linked Data relating to UK Statistics" ;
    foaf:homepage <http://data.gov.uk> ;
    void:sparqlEndpoint <http://services.data.gov.uk/statistics/sparql> ;
    void:exampleResource <http://statistics.data.gov.uk/id/local-authority-district/00AK> ;
    void:uriSpace "http://statistics.data.gov.uk/id/" ;
    void:triples "343733"^^xsd:integer .
[ a sd:Service ;
    sd:endpoint <http://services.data.gov.uk/statistics/sparql> ] .

_:Nature a void:Dataset ;
    dct:title "Nature" ;
    dct:description "The NPG Linked Data Platform provides access to datasets from NPG published as linked data and made available through SPARQL services" ;
    foaf:homepage <http://data.nature.com> ;
    foaf:depiction <http://data.nature.com/view/cerberus/images/header.jpg> ;
    void:sparqlEndpoint <http://data.nature.com/sparql> ;
    void:exampleResource <http://data.nature.com/ns/articles/10.1038/111697a0> ;
    void:uriSpace "http://data.nature.com/" ;
    void:triples "327539066"^^xsd:integer .
[ a sd:Service ;
    sd:endpoint <http://data.nature.com/sparql> ] .

_:BBC a void:Dataset ;
    dct:title "BBC" ;
    foaf:logo <http://upload.wikimedia.org/wikipedia/commons/e/eb/BBC.svg> ;
    void:exampleResource <http://www.bbc.co.uk/programmes/b006t6c5> .

_:Twitter a void:Dataset ;
    dct:title "Twitter" ;
    foaf:homepage <http://twitter.com> ;
    foaf:logo <https://abs.twimg.com/a/1369413260/images/resources/twitter-bird-callout.png> ;
    void:exampleResource <https://api.twitter.com/1/users/show.xml?screen_name=pumba_lt> ,
	<https://api.twitter.com/1/users/show.xml?screen_name=graphityhq> ;
    void:uriSpace "https://api.twitter.com/1/" .

_:EEA a void:Dataset ;
    dct:title "European Environment Agency" ;
    dct:description "Semantic Data Service is an object-oriented search engine where you can search for the content of data in Eionet" ;
    foaf:homepage <http://semantic.eea.europa.eu/> ;
    foaf:depiction <http://wwws4.eea.europa.eu/about-us/documents/logos/eps_logos/eea_mini.gif> ;
    void:sparqlEndpoint <http://semantic.eea.europa.eu/sparql> .

_:SWDogFood a void:Dataset ;
    dct:title "Semantic Web Dog Food Corpus" ;
    dct:description "Information on papers that were presented, people who attended, and other things that have to do with the main conferences and workshops in the area of Semantic Web research" ;
    foaf:homepage <http://data.semanticweb.org/> ;
    foaf:logo <http://data.semanticweb.org/images/bones_small.png> ;
    void:sparqlEndpoint <http://data.semanticweb.org/sparql> ;
    void:exampleResource <http://data.semanticweb.org/conference/dc/2010/paper/main/A-1004> ,
	<http://data.semanticweb.org/organization/w3c> ,
	<http://data.semanticweb.org/person/ora-lassila> ;
    void:triples "221690"^^xsd:integer .
[] a sd:Service ;
    sd:endpoint <http://data.semanticweb.org/sparql> .

_:LinkedMDB a void:Dataset ;
    dct:title "LinkedMDB" ;
    dct:description "The project aims at publishing the first open semantic web database for movies, including a large number of interlinks to several datasets on the open data cloud and references to related webpages." ;
    foaf:homepage <http://data.linkedmdb.org/> ;
    void:sparqlEndpoint <http://data.linkedmdb.org/sparql> ;
    void:exampleResource <http://data.linkedmdb.org/resource/film/2014> ;
    void:uriSpace "http://data.linkedmdb.org/resource/" .
[] a sd:Service ;
    sd:endpoint <http://data.linkedmdb.org/sparql> .

_:Health a void:Dataset ;
    dct:title "Health Data Community" ;
    dct:description "Public resource designed to bring together high-value datasets, tools, and applications using data about health and health care to support your need for better knowledge and to help you to solve problems" ;
    foaf:homepage <http://healthdata.gov> ;
    void:sparqlEndpoint <http://health.data.gov/sparql> ;
    void:exampleResource <http://health.data.gov/id/ahrqp/2011-12-14/recordset/3065/record/19> .
[] a sd:Service ;
    sd:endpoint <http://health.data.gov/sparql> .

_:Commerce a void:Dataset ;
    dct:title "The Linked Open Commerce Dataspace" ;
    dct:description "An Emerging, Open Architecture for Global e-Commerce based on Linked Data" ;
    foaf:homepage <http://linkedopencommerce.com> ;
    void:sparqlEndpoint <http://linkedopencommerce.com/sparql> .
#    void:exampleResource <http://openean.kaufkauf.net/id/businessentities/GLN_6079860000028> ,
#	<http://rdf4ecommerce.esolda.com/camcorder/model_110401#model> .
[] a sd:Service ;
    sd:endpoint <http://linkedopencommerce.com/sparql> .

_:WorldBank a void:Dataset ;
    dct:title "World Bank" ;
    dct:description "This site contains The World Bank data published using the Linked Data design principles" ;
    foaf:homepage <http://worldbank.270a.info> ;
    void:sparqlEndpoint <http://worldbank.270a.info/sparql> ;
    void:exampleResource <http://worldbank.270a.info/classification/country/CA> ,
	<http://worldbank.270a.info/dataset/world-development-indicators> ;
    void:uriSpace "http://worldbank.270a.info/" .
[] a sd:Service ;
    sd:endpoint <http://worldbank.270a.info/sparql> .

_:OpenDataCommunities a void:Dataset ;
    dct:title "Open Data Communities" ;
    dct:description "This site is the Department for Communities and Local Government's first step towards more open, accessible and re-usable data." ;
    foaf:homepage <http://opendatacommunities.org> ;
    void:sparqlEndpoint <http://opendatacommunities.org/sparql> ;
    void:exampleResource <http://opendatacommunities.org/id/housing/homelessness-decisions/2011-Q3/E09000033/rejected-not-priority> .
[] a sd:Service ;
    sd:endpoint <http://opendatacommunities.org/sparql> .

_:SchoolsInDenmark a void:Dataset ;
    dct:title "Schools in Denmark" ;
    dct:description "Dataset with geo-located school information (Denmark only)" ;
    dct:source <http://oiorest.dk/danmark> ;
    # dct:subject <http://dbpedia.org/resource/Denmark> ;
    void:sparqlEndpoint <http://semantic-web.dk/projects/schools/sparql> ;
    void:exampleResource <http://semantic-web.dk/projects/schools/resource/101172> .
[] a sd:Service ;
    sd:endpoint <http://semantic-web.dk/projects/schools/sparql> .

_:Reegle a void:Dataset ;
    dct:title "reegle Data" ;
    dct:description "Energy policy reports for more than 160 countries; clean energy stakeholders; project output documents; more than 3000 clean energy terms from our thesaurus" ;
    foaf:homepage <http://data.reegle.info> ;
    foaf:logo <http://data.reegle.info/images/reegle_data_logo.png> ;
    void:sparqlEndpoint <http://sparql.reegle.info> ;
    void:exampleResource <http://reegle.info/actors/2354> ,
	<http://reegle.info/countries/AT> .
[] a sd:Service ;
    sd:endpoint <http://sparql.reegle.info> .

_:LinkedLifeData a void:Dataset ;
    dct:title "LinkedLifeData" ;
    dct:description "A semantic data integration platform for the biomedical domain" ;
    foaf:homepage <http://linkedlifedata.com> ;
    foaf:logo <http://linkedlifedata.com/img/logo-large.png> ;
    void:sparqlEndpoint <http://linkedlifedata.com/sparql> ;
    void:exampleResource <http://linkedlifedata.com/resource/entrezgene/id/7158> ,
	<http://linkedlifedata.com/resource/drug-target/16> ;
    void:triples "1000000000"^^xsd:integer .
[] a sd:Service ;
    sd:endpoint <http://linkedlifedata.com/sparql> .

# QUERY TEMPLATES

:DescribeTemplate a spin:Template ;
    spin:body :Describe ;
    rdfs:isDefinedBy : .

:Describe    a       sp:Describe ;
      sp:resultNodes (spin:_this _:docVar _:thingVar) ;
      sp:text """PREFIX foaf: <http://xmlns.com/foaf/0.1/>
PREFIX sioc: <http://rdfs.org/sioc/ns#>
DESCRIBE ?this ?doc ?thing WHERE {
    OPTIONAL {
        {
            ?this foaf:primaryTopic ?thing .
        }
        UNION
        {
            ?doc sioc:has_space ?this .
        }
        UNION
        {
            {
PREFIX foaf: <http://xmlns.com/foaf/0.1/>
PREFIX sioc: <http://rdfs.org/sioc/ns#>
                SELECT ?doc ?thing
                WHERE {
                    ?doc sioc:has_container ?this .
                    OPTIONAL {
                        ?doc foaf:primaryTopic ?thing .
                    } .
                }
            } .
        } .
    } .
}"""^^xsd:string ;
      sp:where ([ a       sp:Optional ;
                  sp:elements ([ a       sp:Union ;
                              sp:elements (([ sp:object _:thingVar ;
                                            sp:predicate foaf:primaryTopic ;
                                            sp:subject spin:_this
                                          ]) ([ sp:object spin:_this ;
                                            sp:predicate sioc:has_space ;
                                            sp:subject _:docVar
                                          ]) ([ a       sp:SubQuery ;
                                            sp:query
                                                    [ a       sp:Select ;
                                                      sp:resultVariables (_:docVar _:thingVar) ;
                                                      sp:where ([ sp:object spin:_this ;
                                                                  sp:predicate sioc:has_container ;
                                                                  sp:subject _:docVar
                                                                ] [ a       sp:Optional ;
                                                                  sp:elements ([ sp:object _:thingVar ;
                                                                              sp:predicate foaf:primaryTopic ;
                                                                              sp:subject _:docVar
                                                                            ])
                                                                ])
                                                    ]
                                          ]))
                            ])
                ]) .

_:docVar  sp:varName "doc"^^xsd:string .
_:thingVar  sp:varName "thing"^^xsd:string .